Renames

theories/DSub/unary_lr.v
@@ -33,11 +33,11 @@ Section logrel.
 
   (* XXX this is wrong unless we translate, and here I want for now to switch to having no translation.
      Tho maybe let's do one thing at a time. *)
-  Definition idm_proj_semtype v (φ : D) : iProp Σ :=
+  Definition dm_to_type v (φ : D) : iProp Σ :=
     (∃ γ σ interp, ⌜ v = vstamp σ γ ⌝ ∗ γ ⤇ interp ∗ φ ≡ interp (to_subst σ))%I.
-  Global Arguments idm_proj_semtype /.
-  Notation "v ↗ φ" := (idm_proj_semtype v φ) (at level 20).
-  Global Instance idm_proj_persistent d τ: Persistent (d ↗ τ) := _.
+  Global Arguments dm_to_type /.
+  Notation "v ↗ φ" := (dm_to_type v φ) (at level 20).
+  Global Instance dm_to_type_persistent d τ: Persistent (d ↗ τ) := _.
 
   Definition interp_tmem interp1 interp2 : envD Σ :=
     λ ρ v,
